%
% Copyright Â© 2017 Peeter Joot.  All Rights Reserved.
% Licenced as described in the file LICENSE under the root directory of this GIT repository.
%
We've identified the vector wedge product of two vectors with the selection of the highest grade of their product.
Looking back to the multivector products of \cref{eqn:generalizedDot:601}, and \cref{eqn:generalizedDot:621} as motivation,
a generalized wedge product can be defined that selects the highest grade terms of a given multivector product

\index{multivector wedge product}
\index{\(A \wedge B\)}
\makedefinition{Multivector wedge product.}{dfn:generalizedWedge:480}{
For the multivectors \( A, B \) defined in \cref{dfn:generalizedDot:100}, the wedge (or outer) product is defined as
\begin{equation*}
A \wedge B
\equiv
\sum_{i,j = 0}^N \gpgrade{ A_i B_j }{i + j}.
\end{equation*}
} % definition

If \( A, B \) are a k-vectors with grades \( r, s \) respectively, then their wedge product is a single grade selection
\begin{equation}\label{eqn:generalizedWedge:560}
A \wedge B = \gpgrade{ A B }{ r + s}.
\end{equation}

The most important example of the generalized wedge is the wedge product of a vector with wedge of two vectors

\maketheorem{Wedge of three vectors.}{thm:generalizedWedge:vectorTwoBlade}{
The wedge product of three vectors is associative
\begin{equation*}
(\Ba \wedge \Bb) \wedge \Bc = \Ba \wedge (\Bb \wedge \Bc),
\end{equation*}
so can be written simply as \( \Ba \wedge \Bb \wedge \Bc \).
} % theorem
\begin{proof}
The proof follows directly from the definition
\begin{equation}\label{eqn:generalizedWedge:580}
\begin{aligned}
(\Ba \wedge \Bb) \wedge \Bc
&= \gpgradethree{ (\Ba \wedge \Bb) \Bc } \\
&= \gpgradethree{ (\Ba \Bb -\Ba \cdot \Bb) \Bc } \\
&= \gpgradethree{ \Ba \Bb \Bc } - (\Ba \cdot \Bb) \gpgradethree{ \Bc } \\
&= \gpgradethree{ \Ba \Bb \Bc },
\end{aligned}
\end{equation}
where the grade-3 selection of a vector is zero by definition.
Similarly
\begin{equation}\label{eqn:generalizedWedge:600}
\begin{aligned}
\Ba \wedge (\Bb \wedge \Bc)
&= \gpgradethree{ \Ba (\Bb \wedge \Bc) } \\
&= \gpgradethree{ \Ba (\Bb \Bc - \Bb \cdot \Bc) } \\
&= \gpgradethree{ \Ba \Bb \Bc } - (\Bb \cdot \Bc) \gpgradethree{ \Ba } \\
&= \gpgradethree{ \Ba \Bb \Bc }.
\end{aligned}
\end{equation}
\end{proof}
%which proves the theorem.

It is simple to show that the wedge of three vectors is completely antisymmetric (any interchange of vectors changes the sign), and that cyclic permutation \( \Ba \rightarrow \Bb \rightarrow \Bc \rightarrow \Ba \) of the vectors leaves it unchanged
(\cref{problem:generalizedWedge:tripleWedgeProperties}).
These properties are also common to the scalar triple product of \R{3} vector algebra, because both the scalar triple product and the wedge of three vectors has a determinant structure, which can be shown by direct expansion in coordinates
\begin{equation}\label{eqn:generalizedWedge:620}
\begin{aligned}
\Ba \wedge \Bb \wedge \Bc
&= \gpgradethree{ a_i b_j c_k \Be_i \Be_j \Be_k } \\
&= \sum_{i \ne j \ne k} a_i b_j c_k \Be_i \Be_j \Be_k \\
&= \sum_{i < j < k}
   \begin{vmatrix}
   a_i & a_j & a_k \\
   b_i & b_j & b_k \\
   c_i & c_j & c_k \\
   \end{vmatrix}
   \Be_{i j k}.
\end{aligned}
\end{equation}

In \R{3} this sum has only one term
\begin{equation}\label{eqn:generalizedWedge:680}
\Ba \wedge \Bb \wedge \Bc
=
\begin{vmatrix}
a_1 & a_2 & a_3 \\
b_1 & b_2 & b_3 \\
c_1 & c_2 & c_3 \\
\end{vmatrix}
I,
\end{equation}
in which the determinant is recognizable as the scalar triple product.  This shows that the \R{3} wedge of three vectors is the scalar triple product times the pseudoscalar
\boxedEquation{eqn:generalizedWedge:640}{
\Ba \wedge \Bb \wedge \Bc
=
\lr{ \Ba \cdot (\Bb \cross \Bc) } I.
}
%%%We have just one identity left in the article to find the GA equivalent of, but will split that into two logical pieces.
%%%\makelemma{Dual of triple wedge.}{lemma:vectorcalc:660}{
%%%If \( \Ba, \Bb, \Bc \in \mathbb{R}^3 \) are vectors, then
%%%\begin{equation*}
%%%\Ba \cdot \lr{ \Bb \cross \Bc } = -I \lr{ \Ba \wedge \Bb \wedge \Bc }.
%%%\end{equation*}
%%%} % lemma
%%%\begin{proof}
%%%\begin{equation}\label{eqn:vectorcalc:680}
%%%\begin{aligned}
%%%\Ba \cdot \lr{ \Bb \cross \Bc }
%%%&=
%%%\gpgradezero{
%%%\Ba \lr{ \Bb \cross \Bc }
%%%} \\
%%%&=
%%%\gpgradezero{
%%%\Ba (-I) \lr{ \Bb \wedge \Bc }
%%%} \\
%%%&=
%%%\gpgradezero{
%%%-I \lr{
%%%\Ba \cdot \lr{ \Bb \wedge \Bc }
%%%+
%%%\Ba \wedge \lr{ \Bb \wedge \Bc }
%%%}
%%%} \\
%%%&=
%%%\gpgradezero{
%%%-I \lr{ \Ba \wedge \lr{ \Bb \wedge \Bc } }
%%%} \\
%%%&=
%%%-I \lr{ \Ba \wedge \lr{ \Bb \wedge \Bc } }.
%%%\end{aligned}
%%%\end{equation}
%%%\end{proof}


Note that the wedge of \( n \) vectors is also associative.
A full proof is possible by induction, which won't be done here.
Instead, as a hint of how to proceed if desired,
consider the coordinate expansion of a trivector wedged with a vector
\begin{equation}\label{eqn:generalizedWedge:660}
\begin{aligned}
(\Ba \wedge \Bb \wedge \Bc) \wedge \Bd
&=
\sum_{i \ne j \ne k, l}
\gpgrade{
a_i b_j c_k
\Be_i \Be_j \Be_k
d_l \Be_l
}{4} \\
&=
\sum_{i \ne j \ne k \ne l}
a_i b_j c_k d_l
\Be_i \Be_j \Be_k \Be_l.
\end{aligned}
\end{equation}

This can be rewritten with any desired grouping \( ((\Ba \wedge \Bb) \wedge \Bc) \wedge \Bd = (\Ba \wedge \Bb) \wedge ( \Bc \wedge \Bd) = \Ba \wedge (\Bb \wedge \Bc \wedge \Bd) = \cdots \).
Observe that this can also be put into a determinant form like that of
\cref{eqn:generalizedWedge:620}.
Whenever the number of vectors matches the dimension of the underlying vector space, this will be a single determinant of all the coordinates of the vectors multiplied by the unit pseudoscalar for the vector space.

