%
% Copyright Â© 2023 Peeter Joot.  All Rights Reserved.
% Licenced as described in the file LICENSE under the root directory of this GIT repository.
%
\section{Vector relations.}
For vectors \( \Ba, \Bb, \Bc, \Bd \)

\begin{equation}\label{eqn:helpful:20}
\begin{aligned}
\Ba \Bb &= \Ba \cdot \Bb + \Ba \wedge \Bb \\
        &= \Ba \cdot \Bb + I\lr{ \Ba \cross \Bb}\qquad (\mathbb{R}^3)
\end{aligned}
\end{equation}
\begin{equation}\label{eqn:helpful:40}
\begin{aligned}
\Ba \cdot \Bb &= \inv{2} \lr{ \Ba \Bb + \Bb \Ba } \\
\Ba \wedge \Bb &= \inv{2} \lr{ \Ba \Bb - \Bb \Ba }
\end{aligned}
\end{equation}
\begin{equation}\label{eqn:helpful:60}
\Bb \Ba = -\Ba \Bb + 2 \Ba \cdot \Bb
\end{equation}
\begin{equation}\label{eqn:helpful:80}
\Ba \wedge \Bb
=
\sum_{i < j}
\begin{vmatrix}
a_i & a_j \\
b_i & b_j
\end{vmatrix}
\Be_i \Be_j
\end{equation}
\begin{equation}\label{eqn:helpful:100}
\begin{aligned}
\Ba \cdot \lr{ \Bb \wedge \Bc }
&=
\lr{ \Bc \wedge \Bb } \cdot \Ba
=
( \Ba \cdot \Bb ) \Bc
-( \Ba \cdot \Bc ) \Bb \\
&= \lr{ \Bb \cross \Bc } \cross \Ba\qquad (\mathbb{R}^3)
\end{aligned}
\end{equation}
\begin{equation}\label{eqn:helpful:120}
\begin{aligned}
(\Ba \wedge \Bb) \cdot (\Bc \wedge \Bd)
&=
\lr{ (\Ba \wedge \Bb) \cdot \Bc} \cdot \Bd
=
(\Bb \cdot \Bc) (\Ba \cdot \Bd)
-(\Ba \cdot \Bc)( \Bb \cdot \Bd) \\
&= -(\Ba \cross \Bb) \cdot (\Bc \cross \Bd)\qquad (\mathbb{R}^3)
\end{aligned}
\end{equation}
\begin{equation}\label{eqn:helpful:140}
\begin{aligned}
\Ba
&= \lr{ \Ba \cdot \Bb} \inv{\Bb} + \lr{ \Ba \wedge \Bb} \inv{\Bb} = \Proj_\Bb(\Ba) + \Rej{\Bb}{\Ba} \\
&= \lr{ \Ba \cdot \bcap} \bcap + \lr{ \Ba \wedge \bcap} \bcap \qquad (\mathbb{R}^N) \\
&= \lr{ \Ba \cdot \bcap} \bcap + \bcap \cross \lr{ \Ba \cross \bcap}\qquad (\mathbb{R}^3) \\
\end{aligned}
\end{equation}
\begin{equation}\label{eqn:helpful:160}
\Ba^{-1} = \frac{\Ba}{\Norm{\Ba}^2}
\end{equation}
\begin{equation}\label{eqn:helpful:180}
\begin{aligned}
\Ba \cdot &\lr{ \Bb \wedge \Bc \wedge \Bd} \\
&=
\lr{ \Bb \wedge \Bc \wedge \Bd} \cdot \Ba \\
&=
( \Ba \cdot \Bb ) (\Bc \wedge \Bd)
-( \Ba \cdot \Bc ) (\Bb \wedge \Bd)
+( \Ba \cdot \Bd ) (\Bb \wedge \Bc)
\end{aligned}
\end{equation}
\begin{equation}\label{eqn:helpful:200}
\begin{aligned}
\Ba \cdot &\lr{ \Bb_1 \wedge \Bb_2 \wedge \cdots \wedge \Bb_n } \\
&=
\sum_{i = 1}^n (-1)^i (\Ba \cdot \Bb_i) \lr{ \Bb_1 \wedge \cdots \wedge \Bb_{i-1} \wedge \Bb_{i+1} \wedge \cdots \wedge \Bb_n }
\end{aligned}
\end{equation}
\begin{equation}\label{eqn:helpful:81}
\begin{aligned}
\Ba \wedge \Bb \wedge \Bc
&=
\sum_{i < j < k}
\begin{vmatrix}
a_i & a_j & a_k \\
b_i & b_j & b_k \\
c_i & c_j & c_k \\
\end{vmatrix}
\Be_i \Be_j \Be_k \\
&= \lr{ \Ba \cdot (\Bb \cross \Bc) } I\qquad (\mathbb{R}^3)
\end{aligned}
\end{equation}
\section{Blades.}
For k-blade \( A_k = \Ba_1 \Ba_2 \cdots \Ba_k \), j-blade \( B_j = \Ba_1 \Ba_2 \cdots \Ba_j \), vector \( \Ba \)
\begin{equation}\label{eqn:helpful:240}
A_k^\dagger = (-1)^{k(k-1)/2} A_k
\end{equation}
\begin{equation}\label{eqn:helpful:260}
\begin{aligned}
A_k \cdot \Ba  &= (-1)^{k-1} \Ba \cdot A_k \\
A_k \wedge \Ba &= (-1)^k \Ba \wedge A_k
\end{aligned}
\end{equation}
\begin{equation}\label{eqn:helpful:280}
\begin{aligned}
\Ba \wedge A_k &= \inv{2}\lr{ \Ba A_k + (-1)^k A_k \Ba } \\
\Ba \cdot A_k &= \inv{2}\lr{ \Ba A_k - (-1)^k A_k \Ba }
\end{aligned}
\end{equation}
\begin{equation*}
A_k \cdot \lr{ \Ba \wedge B_j } = \lr{ A_k \cdot \Ba } \cdot B_j\qquad k > j > 0
\end{equation*}

\section{Multivectors.}
\begin{equation}\label{eqn:helpful:300}
\begin{aligned}
A \cdot B &\equiv \sum_{i,j = 0}^N \gpgrade{ A_i B_j }{\Abs{i - j}} \\
A \wedge B &\equiv \sum_{i,j = 0}^N \gpgrade{ A_i B_j }{i + j}
\end{aligned}
\end{equation}
\begin{equation}\label{eqn:helpful:320}
\begin{aligned}
A \rfloor B &= \sum_{i,j = 0}^N \gpgrade{ A_i B_j }{j - i} \\
A \lfloor B &= \sum_{i,j = 0}^N \gpgrade{ A_i B_j }{i - j} \\
A \conj B &= \sum_{i,j = 0}^N \gpgradezero{ A_i B_j }
\end{aligned}
\end{equation}
\section{Vector calculus identities.}

Blade \( A \),
\begin{equation}\label{eqn:helpful:340}
\spacegrad \wedge \lr{ \spacegrad \wedge A } = 0
\end{equation}
\R{3}, scalar \( f \), vector \( \Bf \)
\begin{equation}\label{eqn:helpful:360}
\begin{aligned}
\spacegrad \cross \lr{ \spacegrad f } &= 0 \\
\spacegrad \cdot \lr{ \spacegrad \cross \Bf } &= 0
\end{aligned}
\end{equation}

\begin{equation}\label{eqn:helpful:380}
\begin{aligned}
\spacegrad \lr{ \Ba \cdot \Bb } &= \lr{ \Ba \cdot \spacegrad } \Bb + \lr{ \Bb \cdot \spacegrad } \Ba + \lr{ \spacegrad \wedge \Bb } \cdot \Ba + \lr{ \spacegrad \wedge \Ba } \cdot \Bb \\
&= \lr{ \Ba \cdot \spacegrad } \Bb + \lr{ \Bb \cdot \spacegrad } \Ba + \Ba \cross \lr{ \spacegrad \cross \Bb } + \Bb \cross \lr{ \spacegrad \cross \Ba } \qquad(\mathbb{R}^3)
\end{aligned}
\end{equation}

\begin{equation}\label{eqn:helpful:400}
\begin{aligned}
\spacegrad \cdot \lr{ \Ba \wedge \Bb }
&= \Bb \lr{ \spacegrad \cdot \Ba } - \Ba \lr{ \spacegrad \cdot \Bb } - \lr{ \Bb \cdot \spacegrad } \Ba + \lr{ \Ba \cdot \spacegrad } \Bb \\
&= -\spacegrad \cross \lr{ \Ba \cross \Bb }\qquad(\mathbb{R}^3)
\end{aligned}
\end{equation}


\begin{equation}\label{eqn:helpful:420}
\spacegrad \wedge \lr{ f \lr{ \spacegrad g \wedge \spacegrad h } } = \spacegrad f \wedge \spacegrad g \wedge \spacegrad h
\end{equation}
For \R{3}
\begin{equation}\label{eqn:helpful:440}
\spacegrad \cdot \lr{ f \lr{ \spacegrad g \cross \spacegrad h } } = \spacegrad f \cdot \lr{ \spacegrad g \cross \spacegrad h }
\end{equation}

\begin{equation}\label{eqn:helpful:460}
\spacegrad \wedge \lr{ \Ba \wedge \Bb } = \Bb \wedge \lr{ \spacegrad \wedge \Ba } - \Ba \wedge \lr{ \spacegrad \wedge \Bb }
\end{equation}
For \R{3}
\begin{equation}\label{eqn:helpful:480}
\spacegrad \cdot \lr{ \Ba \cross \Bb } = \Bb \cdot \lr{ \spacegrad \cross \Ba } - \Ba \cdot \lr{ \spacegrad \cross \Bb }
\end{equation}
